more migration to GPT, perhaps complete

LeanCodePrompts/Translate.lean
@@ -44,6 +44,8 @@ def sysPrompt := "You are a coding assistant who translates from natural languag
 
 def makePrompt(query : String)(pairs: Array (String × String)) : Json:= prompt sysPrompt pairs.toList query 
 
+def makeFlipPrompt(query : String)(pairs: Array (String × String)) : Json:= prompt sysPrompt (pairs.toList.map (fun (x, y) => (y, x))) query
+
 def jsonToExprStrArray (json: Json) : TermElabM (Array String) := do
   let outArr : Array String ← 
     match json.getArr? with
@@ -69,6 +71,7 @@ def jsonToExprStrArray (json: Json) : TermElabM (Array String) := do
 end GPT
 
 /-- make prompt from prompt pairs -/
+@[deprecated GPT.makePrompt]
 def makePrompt(prompt : String)(pairs: Array (String × String)) : String := 
       pairs.foldr (fun  (ds, thm) acc => 
         -- acc ++ "/-- " ++ ds ++" -/\ntheorem" ++ thm ++ "\n" ++ "\n"
@@ -81,6 +84,7 @@ theorem "
 
 
 /-- make prompt for reverse translation from prompt pairs -/
+@[deprecated GPT.makeFlipPrompt]
 def makeFlipPrompt(statement : String)(pairs: Array (String × String)) : String := 
       pairs.foldr (fun  (ds, thm) acc => 
 s!"theorem {thm} := 
@@ -405,9 +409,9 @@ def greedyArrayToExpr? (output: Array String) : TermElabM (Option Expr) := do
 /-- reverse translation from `Lean` to natural language -/
 def leanToPrompt (thm: String)(numSim : Nat:= 5)(numKW: Nat := 1)(temp : JsonNumber := 0)(scoreBound: Float := 0.2)(matchBound: Nat := 15)(textField : String := "text") : TermElabM String := do
     let (pairs, _) ← getPromptPairs thm numSim numKW scoreBound matchBound
-    let prompt := makeFlipPrompt thm pairs
+    let prompt := GPT.makeFlipPrompt thm pairs
     -- elabLog prompt
-    let fullJson ← openAIQuery prompt 1 temp
+    let fullJson ← gptQuery prompt 1 temp
     let outJson := 
       (fullJson.getObjVal? "choices").toOption.getD (Json.arr #[])
     let out? := (outJson.getArrVal? 0).bind fun js => js.getObjVal? textField
@@ -418,6 +422,7 @@ def leanToPrompt (thm: String)(numSim : Nat:= 5)(numKW: Nat := 1)(temp : JsonNum
     return outJson.getStr!
 
 /-- reverse translation from `Lean` to natural language -/
+@[deprecated leanToPrompt]
 def statementToDoc (thm: String)(numSim : Nat:= 5)(temp : JsonNumber := 0) : TermElabM String := do
     let (pairs, _) ← getPromptPairsGeneral thm numSim "statement"
     let prompt := makeFlipStatementsPrompt thm pairs
@@ -539,8 +544,6 @@ elab "uncurry2" e:term : term => do
 
 universe u
 
-#eval uncurry2 ({α : Type u} →  (l: List α) →  (a : α) → a = a)
-#eval uncurry2 ({α : Prop} →  [Decidable α] →  (a : α) → a = a)
 
 def translateViewM (s: String) : TermElabM String := do
   let js ← getCodeJson  s
@@ -562,5 +565,4 @@ def translateViewM (s: String) : TermElabM String := do
 def translateViewCore (s: String) : CoreM String := 
   (translateViewM s).run'.run'
 
-#check Array.findSomeM?
 
